Test/SLList.v
@@ -1,0 +1,288 @@
+From SLFun Require Import Util Values SL VProg VProgGhost.
+From Coq   Require Import Lists.List.
+
+Import SLNotations SL.Tactics.
+Import ListNotations.
+Import VProg.Notations.
+
+
+(* Singly linked lists *)
+
+Record lcell_t := mk_lcell {
+  v_data : memdata;
+  v_next : ptr;
+}.
+
+Definition p_data (p : ptr) : ptr := p.
+Definition p_next (p : ptr) : ptr := S p.
+
+Definition lcell (p : ptr) (v : lcell_t) : SLprop.t :=
+  vptr (p_data p) (v_data v) ** vptr (p_next p) (v_next v).
+
+
+Definition lseg_t := list (ptr * memdata).
+
+Definition lseg_entry (l : lseg_t) (sg_next : ptr) : ptr :=
+  match l with
+  | nil         => sg_next
+  | (p, _) :: _ => p
+  end.
+
+Fixpoint lseg_sl (l : lseg_t) (sg_next : ptr) : SLprop.t :=
+  match l with
+  | nil          => SLprop.emp
+  | (p, d) :: cs => lcell p (mk_lcell d (lseg_entry cs sg_next)) ** lseg_sl cs sg_next
+  end.
+
+Definition lseg (entry next : ptr) (v : lseg_t) : SLprop.t :=
+  SLprop.pure (lseg_entry v next = entry) **
+  lseg_sl v next.
+
+Definition llist (p : ptr) : Vprop.p lseg_t :=
+  lseg p NULL.
+Global Arguments llist/.
+
+(* Lemmas *)
+
+Lemma lcell_non_null p v:
+  SLprop.impp (lcell p v) (p <> NULL).
+Proof.
+  unfold lcell, vptr.
+  eapply SLprop.impp_enough.
+  SLprop.split_impp; [apply SLprop.cell_non_null | apply SLprop.impp_True].
+  intro H; apply H.
+Qed.
+
+Lemma lcell_def p:
+  eqv_lemma [lcell p ~>] [vptr (p_data p) ~>; vptr (p_next p) ~>]
+            (fun v => (v_data v, v_next v))
+            (fun dt nx => mk_lcell dt nx).
+Proof.
+  apply intro_eqv_lemma.
+  - intros []; reflexivity.
+  - intros dt nx; cbn; unfold lcell.
+    SL.normalize.
+    reflexivity.
+Qed.
+
+Definition intro_lseg_nil_spec : LDecl ptr unit
+  FOR p FOR tt [] [] True
+  RET _ FOR tt [lseg p p ~> nil] True.
+Proof. Derive. Defined.
+Lemma intro_lseg_nil : intro_lseg_nil_spec.
+Proof.
+  init_lemma p [] _; unfold lseg; SL.normalize.
+  Apply; reflexivity.
+Qed.
+
+Definition elim_lseg_nil_spec : LDecl (ptr * ptr) unit
+  FOR (p0, p1) FOR l [] [lseg p0 p1 ~> l] (l = nil)
+  RET _ FOR tt [] (p0 = p1).
+Proof. Derive. Defined.
+Lemma elim_lseg_nil : elim_lseg_nil_spec.
+Proof.
+  init_lemma (p0, p1) l ->; unfold lseg; SL.normalize.
+  Intro ->; Apply; reflexivity.
+Qed.
+
+Definition intro_lseg_cons_spec : LDecl (ptr * ptr * ptr) unit
+  FOR (p0, p1, pn) FOR (hd, tl) [] [lcell p0 ~> hd; lseg p1 pn ~> tl] (v_next hd = p1)
+  RET _ FOR tt [lseg p0 pn ~> ((p0, v_data hd) :: tl)] True.
+Proof. Derive. Defined.
+Lemma intro_lseg_cons : intro_lseg_cons_spec.
+Proof.
+  init_lemma ((p0, p1), pn) ([], tl) <-.
+  unfold lseg; SL.normalize.
+  Intro ->.
+  Apply; reflexivity.
+Qed.
+
+Definition elim_lseg_cons_spec : LDecl (ptr * ptr) ptr
+  FOR (p0, pn) FOR l [] [lseg p0 pn ~> l] (match l with nil => False | cons _ _ => True end)
+  RET p1 FOR (dt, tl) [lcell p0 ~> (mk_lcell dt p1); lseg p1 pn ~> tl]
+    (match l with nil => False | (p0', dt') :: tl' => p0' = p0 /\ dt = dt' /\ tl = tl' end).
+Proof. Derive. Defined.
+Lemma elim_lseg_cons : elim_lseg_cons_spec.
+Proof.
+  init_lemma (p0, pn) [|[p0' dt] tl] [].
+  unfold lseg; cbn; Intro ->.
+  Apply (lseg_entry tl pn); Apply (dt, (tl, tt)); cbn.
+  Apply. repeat split.
+  SL.normalize.
+  Apply; reflexivity.
+Qed.
+
+Definition elim_llist_nnull_spec : LDecl ptr ptr
+  FOR p0 FOR l [] [llist p0 ~> l] (p0 <> NULL)
+  RET p1 FOR (dt, tl) [lcell p0 ~> (mk_lcell dt p1); llist p1 ~> tl] (l = (p0, dt) :: tl).
+Proof. Derive. Defined.
+Lemma elim_llist_nnull : elim_llist_nnull_spec.
+Proof.
+  init_lemma p0 l NNULL.
+  unfold lseg; Intro <-.
+  destruct l as [|[p0' dt] tl]; cbn in *.
+    { exfalso; apply NNULL; reflexivity. }
+  Apply (lseg_entry tl NULL); Apply (dt, (tl, tt)); cbn.
+  SL.normalize.
+  Apply. repeat split.
+  reflexivity.
+Qed.
+
+Lemma lseg_sl_null_nil l n
+  (N : lseg_entry l n = NULL):
+  SLprop.impp (lseg_sl l n) (l = nil).
+Proof.
+  destruct l as [|[]]; cbn.
+  - apply SLprop.impp_drop. reflexivity.
+  - cbn in N; subst.
+    eapply SLprop.impp_enough.
+    SLprop.split_impp; [apply lcell_non_null | apply SLprop.impp_True].
+    intuition congruence.
+Qed.
+
+Definition lseg_null_nil p pn : impp_lemma (fun l => (
+  [lseg p pn ~> l], (p = NULL),
+  fun _ : unit => l = nil)).
+Proof.
+  apply intro_impp_lemma; intros l ->.
+  unfold lseg; SL.normalize.
+  Intro N.
+  eapply SLprop.impp_enough. apply lseg_sl_null_nil, N.
+  exists tt; tauto.
+Qed.
+
+Lemma lseg_entry_app l0 l1 p2:
+  lseg_entry (l0 ++ l1) p2 = lseg_entry l0 (lseg_entry l1 p2).
+Proof.
+  case l0; reflexivity.
+Qed.
+
+Lemma lseg_sl_app l0 l1 p2:
+  SLprop.eq (lseg_sl (l0 ++ l1) p2) (lseg_sl l0 (lseg_entry l1 p2) ** lseg_sl l1 p2).
+Proof.
+  induction l0 as [|[] l0 IH]; cbn.
+  - SL.normalize; reflexivity.
+  - rewrite IH, lseg_entry_app.
+    SL.normalize; reflexivity.
+Qed.
+
+Definition lseg_app_spec : LDecl (ptr * ptr * ptr) unit
+  FOR (p0, p1, p2) FOR (l0, l1) [] [lseg p0 p1 ~> l0; lseg p1 p2 ~> l1] True
+  RET _ FOR tt [lseg p0 p2 ~> (l0 ++ l1)] True.
+Proof. Derive. Defined.
+Lemma lseg_app : lseg_app_spec.
+Proof.
+  init_lemma ((p0, p1), p2) (l0, l1) _.
+  unfold lseg.
+  rewrite lseg_entry_app, lseg_sl_app; SL.normalize.
+  Intro [<- <-].
+  Apply; reflexivity.
+Qed.
+
+
+(* Implementation *)
+
+Section Program.
+  Variables (SIG : sig_context) (SPEC : ConcreteProg.spec_context SIG).
+
+Definition Length_spec : FDecl ptr _ nat _
+  FOR p
+  FOR l [llist p ~> l] [] True
+  RET n FOR tt [] (n = length l).
+Proof. Derive. Defined.
+Variable Length : Length_spec _ SPEC.
+
+Definition Length_impl : FImpl Length := fun p0 =>
+  if Mem.ptr_eq p0 NULL
+  then
+    gLem (lseg_null_nil p0 NULL) tt;;
+    Ret 0
+  else
+    'g_p1 <- gLem elim_llist_nnull p0;
+    gUnfold (lcell_def p0);;
+    'p1 <- Read (p_next p0);
+    gFold (lcell_def p0);;
+    gLem replace1 (llist g_p1, llist p1);;
+    (* ALT: gLem (replace [llist g_p1~>] [llist p1~>]) eq_refl;; *)
+    'n  <- Length p1;
+    gLem intro_lseg_cons (p0, p1, NULL);;
+    Ret (S n).
+Lemma Length_correct : FCorrect Length_impl.
+Proof. by_wlp. Qed.
+Definition Length_cp : f_extract Length_impl.
+Proof. Derive. Defined.
+
+Definition Rev_spec : FDecl (ptr * ptr) _ ptr _
+  FOR (p, pr)
+  FOR l [] [llist p ~> l] True
+  RET r FOR tt [lseg r pr ~> rev l] True.
+Proof. Derive. Defined.
+Variable Rev : Rev_spec _ SPEC.
+
+Definition Rev_impl : FImpl Rev := fun '(p0, pr) =>
+  gLem intro_lseg_nil pr;;
+  if Mem.ptr_eq p0 NULL
+  then
+    gLem (lseg_null_nil p0 NULL) tt;;
+    gLem elim_lseg_nil (p0, NULL);;
+    Ret pr (pt := fun r => [lseg r pr ~>])
+  else
+    'g_p1 <- gLem elim_llist_nnull p0;
+    gUnfold (lcell_def p0);;
+    'p1 <- Read (p_next p0);
+    Write (p_next p0) pr;;
+    gFold (lcell_def p0);;
+    gLem replace1 (llist g_p1, llist p1);;
+    gLem intro_lseg_cons (p0, pr, pr);;
+    'r <- Rev (p1, p0);
+    gLem lseg_app (r, p0, pr);;
+    Ret r (pt := fun r => [lseg r pr ~>]).
+Lemma Rev_correct : FCorrect Rev_impl.
+Proof. by_wlp. Qed.
+Definition Rev_cp : f_extract Rev_impl.
+Proof. Derive. Defined.
+End Program.
+
+Section Extraction.
+  Definition SIG : sig_context :=
+    fun f => match f with
+    | 0 => Some (fd_sig Length_spec)
+    | 1 => Some (fd_sig Rev_spec)
+    | _ => None
+    end.
+
+  Definition SPEC : ConcreteProg.spec_context SIG :=
+    fun f => match f with
+    | 0 => fd_cp Length_spec
+    | 1 => fd_cp Rev_spec
+    | _ => tt
+    end.
+
+  Definition H_Length := fd_mk 0 Length_spec SPEC eq_refl eq_refl.
+  Definition H_Rev    := fd_mk 1 Rev_spec    SPEC eq_refl eq_refl.
+
+  Definition IMPL : ConcreteProg.impl_context SIG :=
+    fun f => match f with
+    | 0 => proj1_sig (Length_cp _ _ H_Length)
+    | 1 => proj1_sig (Rev_cp    _ _ H_Rev)
+    | _ => tt
+    end.
+
+  Lemma match_context:
+    ConcreteProg.context_match_spec IMPL SPEC.
+  Proof.
+    Tac.case_until_True;
+    cbn beta iota delta [SIG IMPL SPEC];
+    apply f_extract_match_spec.
+    - apply Length_correct.
+    - apply Rev_correct.
+  Qed.
+
+  Lemma context_oracle_free:
+    ConcreteProg.context_oracle_free IMPL.
+  Proof.
+    Tac.case_until_True;
+    cbn beta iota delta [SIG IMPL SPEC];
+    apply f_extract_oracle_free.
+  Qed.
+End Extraction.
