VProgGhost.v
@@ -1,0 +1,141 @@
+From SLFun Require Import Util Values SL VProg.
+From Coq   Require Import Lists.List.
+
+Import SLNotations SL.Tactics.
+Import ListNotations.
+Import VProg.Notations.
+
+Section Admit.
+  Lemma admit_change {A} : @ghost_lem (mk_f_sig (VpropList.t * (A -> VpropList.t)) A)
+    (fun '(V0, V1) _ =>
+     Spec.mk_r0 (Tuple.force_match (VpropList.sel V0) (fun sel0 =>
+     Spec.mk_r1 (GO := None) [] (VpropList.inst V0 sel0) False (fun x =>
+     Spec.mk_r2 _ (V1 x) (Tuple.of_fun (fun sel1 =>
+     Spec.mk_r3 _ sel1 True)))))).
+  Proof.
+    init_lemma (?, ?) ?.
+    rewrite Tuple.to_of_fun; intros [].
+  Qed.
+End Admit.
+Section Equivalence.
+  Variables (V0 V1 : VpropList.t).
+  Section Proof.
+    Variables (f : VpropList.sel_t V0 -> VpropList.sel_t V1) (g : VpropList.sel_t V1 -> VpropList.sel_t V0).
+
+    Definition eqv_lem1_spec : ghost_spec (mk_f_sig unit unit) :=
+      fun _ _ =>
+      Spec.mk_r0 (Tuple.force_match (VpropList.sel V0) (fun sel0 =>
+      Spec.mk_r1 [] (VpropList.inst V0 sel0) True (fun _ =>
+      Spec.mk_r2 [] V1 (
+      Spec.mk_r3 _ (f sel0) True)))).
+    
+    Definition eqv_lem2_spec : ghost_spec (mk_f_sig unit unit) :=
+      fun _ _ =>
+      Spec.mk_r0 (Tuple.force_match (VpropList.sel V1) (fun sel1 =>
+      Spec.mk_r1 [] (VpropList.inst V1 sel1) True (fun _ =>
+      Spec.mk_r2 [] V0 (
+      Spec.mk_r3 _ (g sel1) True)))).
+
+    Hypothesis (GF : forall x, g (f x) = x)
+               (E : forall y, SLprop.eq (CTX.sl (VpropList.inst V0 (g y))) (CTX.sl (VpropList.inst V1 y))).
+ 
+    Lemma eqv_lem1 : ghost_lem eqv_lem1_spec.
+    Proof.
+      init_lemma _ sel0 _.
+      rewrite Tuple.to_of_fun; cbn; SL.normalize.
+      rewrite !CTX.sl_app, <- E, GF.
+      reflexivity.
+    Qed.
+    
+    Lemma eqv_lem2 : ghost_lem eqv_lem2_spec.
+    Proof.
+      init_lemma _ sel1 _.
+      rewrite Tuple.to_of_fun; cbn; SL.normalize.
+      rewrite !CTX.sl_app, E.
+      reflexivity.
+    Qed.
+  End Proof.
+
+  Variables
+    (f : Tuple.arrow (VpropList.sel V0) (fun _ => Tuple.u_t (VpropList.sel V1)))
+    (g : Tuple.arrow (VpropList.sel V1) (fun _ => Tuple.u_t (VpropList.sel V0))).
+
+  Let f' x := Tuple.of_u_t (Tuple.to_fun f x).
+  Let g' x := Tuple.of_u_t (Tuple.to_fun g x).
+
+  Definition eqv_lemma : Prop :=
+    ghost_lem (eqv_lem1_spec f') /\ ghost_lem (eqv_lem2_spec g').
+
+  Lemma intro_eqv_lemma
+    (GF : Tuple.arrow (VpropList.sel V0) (fun sel0 => g' (f' sel0) = sel0))
+    (E  : Tuple.arrow (VpropList.sel V1) (fun sel1 =>
+            SLprop.eq (CTX.sl (VpropList.inst V0 (g' sel1)))
+                      (CTX.sl (VpropList.inst V1 sel1))))
+    : eqv_lemma.
+  Proof.
+    specialize (Tuple.to_fun GF) as GF'.
+    specialize (Tuple.to_fun  E) as E'.
+    split; eauto using eqv_lem1, eqv_lem2.
+  Qed.
+
+  Definition gUnfold {SIG SPC} (L : eqv_lemma) : @instr SIG SPC unit :=
+    gLem (proj1 L) tt.
+  Definition gFold {SIG SPC} (L : eqv_lemma) : @instr SIG SPC unit :=
+    gLem (proj2 L) tt.
+End Equivalence.
+Global Arguments gUnfold [_ _ _ _] {_ _} L.
+Global Arguments gFold   [_ _ _ _] {_ _} L.
+Section Replace.
+  Definition replace1_spec A : LDecl (Vprop.p A * Vprop.p A) unit
+    FOR (v0, v1) FOR x [] [v0 ~> x] (v0 = v1)
+    RET _ FOR tt [v1 ~> x] True.
+  Proof. Derive. Defined.
+  Lemma replace1 {A} : replace1_spec A.
+  Proof.
+    init_lemma (v0, v1) sel0 E; subst; reflexivity.
+  Qed.
+
+  Definition replace (V0 V1 : VpropList.t) : @ghost_lem (mk_f_sig (VpropList.sel V0 = VpropList.sel V1) unit)
+    (fun E _ =>
+     Spec.mk_r0 (Tuple.force_match (VpropList.sel V0) (fun sel0 =>
+     Spec.mk_r1 [] (VpropList.inst V0 sel0)
+       (eq_rect _ (fun st => Tuple.t st -> CTX.t) (VpropList.inst V0) _ E = VpropList.inst V1) (fun _ =>
+     Spec.mk_r2 [] V1 (
+     Spec.mk_r3 _ (eq_rect _ Tuple.t sel0 _ E) True))))).
+  Proof.
+    init_lemma E sel0.
+    rewrite Tuple.to_of_fun; cbn.
+    intros <-.
+    SL.normalize.
+    destruct E; cbn; reflexivity.
+  Qed.
+End Replace.
+Section Impp.
+  Context [sel_t A : Type] (spc : sel_t -> (CTX.t * Prop * (A -> Prop))).
+
+  Definition impp_lemma_spec : ghost_spec (mk_f_sig unit A) :=
+      fun _ _ =>
+      Spec.mk_r0 (fun (sel : sel_t) => let '(sl, pre, post) := spc sel in
+      Spec.mk_r1 (GO := None) sl [] pre (fun (x : A) =>
+      Spec.mk_r2 [] [] (
+      Spec.mk_r3 [] tt (post x)))).
+
+  Definition impp_lemma := ghost_lem impp_lemma_spec.
+
+  Lemma intro_impp_lemma
+    (H : forall sel : sel_t, let '(sl, pre, post) := spc sel in
+         pre -> SLprop.impp (CTX.sl sl) (exists x : A, post x)):
+    impp_lemma.
+  Proof.
+    unfold impp_lemma.
+    init_lemma [] sel PRE.
+    specialize (H sel).
+    destruct (spc sel) as ((sl, pre), post); cbn in *.
+    SL.normalize.
+    eapply SLprop.cut_pure. apply H, PRE.
+    intros [x POST].
+    Apply x.
+    Apply POST.
+    reflexivity.
+  Qed.
+End Impp.
